Tests.lean
@@ -9,6 +9,7 @@ import Tests.Direction
 import Tests.Examples
 import Tests.Grid
 import Tests.Invariance
+import Tests.Memory
 import Tests.Output
 import Tests.Parser
 import Tests.Random
