Tests/Memory.lean
@@ -1,0 +1,47 @@
+/-
+Copyright (c) 2026 Bangyen Pham. All rights reserved.
+Released under Apache 2.0 license as described in the file LICENSE.
+Authors: Bangyen Pham
+-/
+import LeanFunge.Theory.Memory
+
+/-!
+# Memory Model Tests
+-/
+
+namespace LeanFunge.Tests
+
+open LeanFunge LeanFunge.Examples
+
+example : gridNoPut quineGrid :=
+  quine_gridNoPut
+
+example (n : ℕ) (s' : State 45 1) (h : run n quineState = some s') :
+    s'.grid = quineGrid :=
+  quine_grid_invariant n s' h
+
+example : runWrites 8 selfmodState = [selfmodWrite] :=
+  selfmod_runWrites
+
+example (s : State 10 1) (h : run 8 selfmodState = some s) :
+    s.grid = Grid.put selfmodGrid 8 0 '@' :=
+  selfmod_grid s h
+
+example (s : State 10 1) (h : run 8 selfmodState = some s) (x y : ℕ)
+    (hne : x % 10 ≠ 8 % 10 ∨ y % 1 ≠ 0 % 1) :
+    s.grid.get x y = selfmodGrid.get x y :=
+  selfmod_grid_other s h x y hne
+
+example : runWrites 7 execState = [execWrite] :=
+  exec_runWrites
+
+example (s : State 10 1) (h : run 7 execState = some s) :
+    s.grid = Grid.put execGrid 7 0 '1' :=
+  exec_grid s h
+
+example (s : State 10 1) (h : run 7 execState = some s) (x y : ℕ)
+    (hne : x % 10 ≠ 7 % 10 ∨ y % 1 ≠ 0 % 1) :
+    s.grid.get x y = execGrid.get x y :=
+  exec_grid_other s h x y hne
+
+end LeanFunge.Tests
